@base <http://www.opencadc.org/caom2/ProductType>.
@prefix : <#>.

@prefix dc: <http://purl.org/dc/terms/> .
@prefix rdfs: <http://www.w3.org/2000/01/rdf-schema#> .
@prefix owl: <http://www.w3.org/2002/07/owl#> .
@prefix xsd: <http://www.w3.org/2001/XMLSchema#> .
@prefix rdf: <http://www.w3.org/1999/02/22-rdf-syntax-ns#> .
@prefix foaf: <http://xmlns.com/foaf/0.1/>.

<> a owl:Ontology;
  dc:created "2019-04-04";
  dc:creator [ foaf:name "Patrick Dowler" ];
  rdfs:label "ProductType vocabulary"@en;
  dc:title "ProductType vocabulary"@en;
  dc:description """<div>
Terms from the vocabulary may be used in CAOM instances as values of the 
caom2:Artifact.productType field. Terms in the base vocabulary are to be
used without the URI prefix (e.g. science instead of http://www.opencadc.org/caom2/productType#science).
</div>
""".

dc:created a owl:AnnotationProperty.
dc:creator a owl:AnnotationProperty.
dc:title a owl:AnnotationProperty.
dc:description a owl:AnnotationProperty.

<#science> a rdf:Property;
  rdfs:label "science data";
  rdfs:comment "primary data file for observations that contains the science data (extraterrestrial photons)".

<#calibration> a rdf:Property;
  rdfs:label "calibration data";
  rdfs:comment "primary file for observations intended for use in removing instrument signature".

<#bias> a rdf:Property;
  rdfs:subPropertyOf <#calibration>;
  rdfs:label "bias frame";
  rdfs:comment "calibration file used to correct for CCD bias".

<#dark> a rdf:Property;
  rdfs:subPropertyOf <#calibration>;
  rdfs:label "dark frame";
  rdfs:comment "calibration file used to correct for no exposure counts in a CCD readout".

<#flat> a rdf:Property;
  rdfs:subPropertyOf <#calibration>;
  rdfs:label "flat field";
  rdfs:comment "calibration file used to correct for sensitivity variation across a CCD".

<#auxiliary> a rdf:Property;
  rdfs:label "related file";
  rdfs:comment "file that could be useful in interpreting the primary file(s)".

<#noise> a rdf:Property;
  rdfs:subPropertyOf <#auxiliary>;
  rdfs:label "noise map";
  rdfs:comment "auxiliary file that provides noise estimates per pixel in the primary file(s)".

<#weight> a rdf:Property;
  rdfs:subPropertyOf <#auxiliary>;
  rdfs:label "weight map";
  rdfs:comment "auxiliary file that provides weights that can be used when analysing the primary file(s)".

<#info> a rdf:Property;
  rdfs:label "human-readable information";
  rdfs:comment "extra information about the primary files (e.g. processing logs)".

<#preview> a rdf:Property;
  rdfs:label "preview image";
  rdfs:comment "a degraded representation of the data useful for display and assessing content".

<#thumbnail> a rdf:Property;
  rdfs:subPropertyOf <#preview>;
  rdfs:label "small preview image";
  rdfs:comment "a highly degraded representation of the data suitable for displaying in a list".

